Update internship_machine.thy

internship_machine.thy
@@ -1,5 +1,6 @@
 theory internship_machine
   imports Main
+
 begin
 
 datatype State = S_1 | S_2 
@@ -23,9 +24,42 @@ fun t:: "State \<times> INPUT \<Rightarrow> State \<times> OUT" where
 "t (S_2, 0) = (S_1, False) "|
 "t (S_2, n) = (S_2, True)"
 
-
+definition INITIAL_NODE:: State where
+"INITIAL_NODE = S_1"
+(* Mesh topology properties*)
 lemma no_dead_ends: "\<forall>s \<in> \<Sigma>. \<exists>i j. fst(t(s,i)) = j"
   by auto
+
+
+  (*check whether there is a path leading between two nodes*)
+inductive path::"nat list \<Rightarrow> State \<Rightarrow> State \<Rightarrow> bool" where
+"fst(t (initial, i)) = current \<Longrightarrow> path [i] initial current"|
+"path [i] initial node \<Longrightarrow> path is node current  \<Longrightarrow> path (i#is) initial current"
+
+
+   (*general path through mesh from the initial node*)
+inductive valid_path::"nat \<Rightarrow> STEP \<Rightarrow> bool" where
+"valid_path 0 \<lparr>INPUT = i, STATE = INITIAL_NODE, OUT = snd(t(S_1, i))\<rparr>"|
+"\<exists>i::nat. valid_path n \<lparr>INPUT = i, STATE = s, OUT = snd(t(s,i))\<rparr> \<Longrightarrow> valid_path (Suc n) \<lparr> INPUT = j, STATE = fst(t(s,i)), OUT = snd(t(fst(t(s,i)), j)) \<rparr>"
+
+  (*Node is cyclic, if there is at least one such path in which it features more than once.*)
+inductive cyclic_node:: "State \<Rightarrow> bool" where
+"path n node node \<Longrightarrow>  cyclic_node node"
+
+inductive cyclic_group::"State list \<Rightarrow> bool" where
+"\<forall>l\<in>(set ls). cyclic_node l \<Longrightarrow> cyclic_group ls"
+
+inductive cyclic_machine:: "bool" where
+"\<forall>n\<in>\<Sigma>. cyclic_node n \<Longrightarrow> cyclic_machine"
+
+inductive not_a_trap_group:: "State set \<Rightarrow> bool" where
+"\<exists>node\<in>grp. \<exists>onode\<in>(\<Sigma>-grp). path i  node onode \<Longrightarrow> not_a_trap_group grp"
+
+inductive trap_group::"State set \<Rightarrow> bool" where
+"\<not>(not_a_trap_group grp)\<Longrightarrow>trap_group grp"
+
+inductive trap_node::"State \<Rightarrow> bool" where
+"trap_group (set[st]) \<Longrightarrow>trap_node st"
 
 
 (*set of all paths*)
@@ -33,50 +67,33 @@ definition paths:: "(nat \<Rightarrow> STEP) set" where
 "paths \<equiv> {p::(nat \<Rightarrow> STEP). STATE(p(0)) = S_1 \<and> (\<forall>n. \<exists>i. t(STATE(p n),i) = (STATE(p(Suc(n))), OUT(p n)))}"
 
 (*very simple S_1 loop*)
-definition path:: "nat \<Rightarrow> STEP" where
-"path n = \<lparr> INPUT = 0,STATE = S_1,OUT = False \<rparr>"
+definition specific_path:: "nat \<Rightarrow> STEP" where
+"specific_path n = \<lparr> INPUT = 0,STATE = S_1,OUT = False \<rparr>"
 
 
-lemma path_init: "STATE(path(0)) = S_1"
-  by (simp add: path_def)
+lemma specific_path_init: "STATE(specific_path(0)) = S_1"
+  by (simp add: specific_path_def)
 
-lemma rhs_simp [simp]: " (STATE(path(Suc(n))), OUT(path n)) = (S_1, False)" using path_def by simp
+lemma rhs_simp [simp]: " (STATE(specific_path(Suc(n))), OUT(specific_path n)) = (S_1, False)" using specific_path_def by simp
 
 
-lemma path_induct: "(\<forall>n. \<exists>i. t(STATE(path n),i) = (STATE(path(Suc(n))), OUT(path n)))"
+lemma path_induct: "(\<forall>n. \<exists>i. t(STATE(specific_path n),i) = (STATE(specific_path(Suc(n))), OUT(specific_path n)))"
 proof (rule allI)
   fix n
-  have 0: "t(STATE(path n), 0) = (STATE(path(Suc(n))), OUT(path n))" using path_def by simp
-  then show "\<exists>i. t (STATE (path n), i) = (STATE (path (Suc n)), OUT (path n))" using exI by simp
+  have 0: "t(STATE(specific_path n), 0) = (STATE(specific_path(Suc(n))), OUT(specific_path n))" using specific_path_def by simp
+  then show "\<exists>i. t (STATE (specific_path n), i) = (STATE (specific_path (Suc n)), OUT (specific_path n))" using exI by simp
 qed
 
-lemma path_in_paths: "path \<in> paths" using path_induct path_init paths_def
+lemma path_in_paths: "specific_path \<in> paths" using path_induct specific_path_init paths_def
   by blast
 
 
 lemma "paths \<noteq> {}" using path_in_paths
   by blast
 
-
-(*check whether there is a path leading between stuffs*)
-inductive route::"nat list \<Rightarrow> State \<Rightarrow> State \<Rightarrow> bool" where
-"fst(t (initial, i)) = current \<Longrightarrow> route [i] initial current"|
-"route [i] initial node \<Longrightarrow> route is node current  \<Longrightarrow> route (i#is) initial current"
-
-(*general path*)
-inductive p::"nat \<Rightarrow> STEP \<Rightarrow> bool" where
-"p 0 \<lparr>INPUT = i, STATE = S_1, OUT = snd(t(S_1, i))\<rparr>"|
-"\<exists>i::nat. p n \<lparr>INPUT = i, STATE = s, OUT = snd(t(s,i))\<rparr> \<Longrightarrow> p (Suc n) \<lparr> INPUT = j, STATE = fst(t(s,i)), OUT = snd(t(fst(t(s,i)), j)) \<rparr>"
-
 lemma big_fish: "\<forall>q\<in>paths. \<forall>m. \<exists>n>m. \<exists>s_0. OUT(q n) = s_0" by auto
 
 
-lemma security: "\<forall>q \<in> paths. \<forall>S \<in> \<Sigma>. \<forall> m. q m = \<lparr>INPUT=1,STATE=S, OUT=True\<rparr>"
-proof
-
-  
-  
- 
-qed
+lemma security: "\<forall>q \<in> paths. \<forall>S \<in> \<Sigma>. \<forall> m. q m = \<lparr>INPUT=1,STATE=S, OUT=True\<rparr>" sorry
 
 end
